fix in progress

src/ocaml-output/FStar_Interactive_PushHelper.ml
@@ -103,6 +103,8 @@ let (set_check_kind :
           (env.FStar_TypeChecker_Env.universe_of);
         FStar_TypeChecker_Env.typeof_well_typed_tot_or_gtot_term =
           (env.FStar_TypeChecker_Env.typeof_well_typed_tot_or_gtot_term);
+        FStar_TypeChecker_Env.subtype_nosmt_force =
+          (env.FStar_TypeChecker_Env.subtype_nosmt_force);
         FStar_TypeChecker_Env.use_bv_sorts =
           (env.FStar_TypeChecker_Env.use_bv_sorts);
         FStar_TypeChecker_Env.qtbl_name_and_index =
