src/ocaml-output/FStar_Tactics_Hooks.ml
@@ -848,6 +848,8 @@ let rec (traverse_for_spinoff :
                              FStar_TypeChecker_Env.typeof_well_typed_tot_or_gtot_term
                                =
                                (env2.FStar_TypeChecker_Env.typeof_well_typed_tot_or_gtot_term);
+                             FStar_TypeChecker_Env.subtype_nosmt_force =
+                               (env2.FStar_TypeChecker_Env.subtype_nosmt_force);
                              FStar_TypeChecker_Env.use_bv_sorts =
                                (env2.FStar_TypeChecker_Env.use_bv_sorts);
                              FStar_TypeChecker_Env.qtbl_name_and_index =
