src/ocaml-output/FStar_Tactics_Types.ml
@@ -309,6 +309,8 @@ let (goal_of_implicit :
             (env.FStar_TypeChecker_Env.universe_of);
           FStar_TypeChecker_Env.typeof_well_typed_tot_or_gtot_term =
             (env.FStar_TypeChecker_Env.typeof_well_typed_tot_or_gtot_term);
+          FStar_TypeChecker_Env.subtype_nosmt_force =
+            (env.FStar_TypeChecker_Env.subtype_nosmt_force);
           FStar_TypeChecker_Env.use_bv_sorts =
             (env.FStar_TypeChecker_Env.use_bv_sorts);
           FStar_TypeChecker_Env.qtbl_name_and_index =
