src/ocaml-output/FStar_Tests_Pars.ml
@@ -80,7 +80,8 @@ let (init_once : unit -> unit) =
         FStar_TypeChecker_TcTerm.tc_term
         FStar_TypeChecker_TcTerm.typeof_tot_or_gtot_term
         FStar_TypeChecker_TcTerm.typeof_tot_or_gtot_term_fastpath
-        FStar_TypeChecker_TcTerm.universe_of solver
+        FStar_TypeChecker_TcTerm.universe_of
+        FStar_TypeChecker_Rel.subtype_nosmt_force solver
         FStar_Parser_Const.prims_lid
         FStar_TypeChecker_NBE.normalize_for_unit_test in
     (env.FStar_TypeChecker_Env.solver).FStar_TypeChecker_Env.init env;
@@ -146,6 +147,8 @@ let (init_once : unit -> unit) =
                (env.FStar_TypeChecker_Env.universe_of);
              FStar_TypeChecker_Env.typeof_well_typed_tot_or_gtot_term =
                (env.FStar_TypeChecker_Env.typeof_well_typed_tot_or_gtot_term);
+             FStar_TypeChecker_Env.subtype_nosmt_force =
+               (env.FStar_TypeChecker_Env.subtype_nosmt_force);
              FStar_TypeChecker_Env.use_bv_sorts =
                (env.FStar_TypeChecker_Env.use_bv_sorts);
              FStar_TypeChecker_Env.qtbl_name_and_index =
@@ -246,6 +249,8 @@ let (init_once : unit -> unit) =
                     (env2.FStar_TypeChecker_Env.universe_of);
                   FStar_TypeChecker_Env.typeof_well_typed_tot_or_gtot_term =
                     (env2.FStar_TypeChecker_Env.typeof_well_typed_tot_or_gtot_term);
+                  FStar_TypeChecker_Env.subtype_nosmt_force =
+                    (env2.FStar_TypeChecker_Env.subtype_nosmt_force);
                   FStar_TypeChecker_Env.use_bv_sorts =
                     (env2.FStar_TypeChecker_Env.use_bv_sorts);
                   FStar_TypeChecker_Env.qtbl_name_and_index =
@@ -389,6 +394,8 @@ let (tc' :
           (tcenv.FStar_TypeChecker_Env.universe_of);
         FStar_TypeChecker_Env.typeof_well_typed_tot_or_gtot_term =
           (tcenv.FStar_TypeChecker_Env.typeof_well_typed_tot_or_gtot_term);
+        FStar_TypeChecker_Env.subtype_nosmt_force =
+          (tcenv.FStar_TypeChecker_Env.subtype_nosmt_force);
         FStar_TypeChecker_Env.use_bv_sorts =
           (tcenv.FStar_TypeChecker_Env.use_bv_sorts);
         FStar_TypeChecker_Env.qtbl_name_and_index =
@@ -484,6 +491,8 @@ let (tc_nbe_term : FStar_Syntax_Syntax.term -> FStar_Syntax_Syntax.term) =
           (tcenv.FStar_TypeChecker_Env.universe_of);
         FStar_TypeChecker_Env.typeof_well_typed_tot_or_gtot_term =
           (tcenv.FStar_TypeChecker_Env.typeof_well_typed_tot_or_gtot_term);
+        FStar_TypeChecker_Env.subtype_nosmt_force =
+          (tcenv.FStar_TypeChecker_Env.subtype_nosmt_force);
         FStar_TypeChecker_Env.use_bv_sorts =
           (tcenv.FStar_TypeChecker_Env.use_bv_sorts);
         FStar_TypeChecker_Env.qtbl_name_and_index =
