src/ocaml-output/FStar_TypeChecker_Tc.ml
@@ -80,6 +80,8 @@ let (set_hint_correlator :
               (env.FStar_TypeChecker_Env.universe_of);
             FStar_TypeChecker_Env.typeof_well_typed_tot_or_gtot_term =
               (env.FStar_TypeChecker_Env.typeof_well_typed_tot_or_gtot_term);
+            FStar_TypeChecker_Env.subtype_nosmt_force =
+              (env.FStar_TypeChecker_Env.subtype_nosmt_force);
             FStar_TypeChecker_Env.use_bv_sorts =
               (env.FStar_TypeChecker_Env.use_bv_sorts);
             FStar_TypeChecker_Env.qtbl_name_and_index = uu___1;
@@ -184,6 +186,8 @@ let (set_hint_correlator :
               (env.FStar_TypeChecker_Env.universe_of);
             FStar_TypeChecker_Env.typeof_well_typed_tot_or_gtot_term =
               (env.FStar_TypeChecker_Env.typeof_well_typed_tot_or_gtot_term);
+            FStar_TypeChecker_Env.subtype_nosmt_force =
+              (env.FStar_TypeChecker_Env.subtype_nosmt_force);
             FStar_TypeChecker_Env.use_bv_sorts =
               (env.FStar_TypeChecker_Env.use_bv_sorts);
             FStar_TypeChecker_Env.qtbl_name_and_index = uu___1;
@@ -1118,6 +1122,8 @@ let (tc_sig_let :
                           FStar_TypeChecker_Env.typeof_well_typed_tot_or_gtot_term
                             =
                             (env1.FStar_TypeChecker_Env.typeof_well_typed_tot_or_gtot_term);
+                          FStar_TypeChecker_Env.subtype_nosmt_force =
+                            (env1.FStar_TypeChecker_Env.subtype_nosmt_force);
                           FStar_TypeChecker_Env.use_bv_sorts =
                             (env1.FStar_TypeChecker_Env.use_bv_sorts);
                           FStar_TypeChecker_Env.qtbl_name_and_index =
@@ -1292,6 +1298,9 @@ let (tc_sig_let :
                                        FStar_TypeChecker_Env.typeof_well_typed_tot_or_gtot_term
                                          =
                                          (env'.FStar_TypeChecker_Env.typeof_well_typed_tot_or_gtot_term);
+                                       FStar_TypeChecker_Env.subtype_nosmt_force
+                                         =
+                                         (env'.FStar_TypeChecker_Env.subtype_nosmt_force);
                                        FStar_TypeChecker_Env.use_bv_sorts =
                                          (env'.FStar_TypeChecker_Env.use_bv_sorts);
                                        FStar_TypeChecker_Env.qtbl_name_and_index
@@ -1645,6 +1654,8 @@ let (tc_decl' :
                      FStar_TypeChecker_Env.typeof_well_typed_tot_or_gtot_term
                        =
                        (env.FStar_TypeChecker_Env.typeof_well_typed_tot_or_gtot_term);
+                     FStar_TypeChecker_Env.subtype_nosmt_force =
+                       (env.FStar_TypeChecker_Env.subtype_nosmt_force);
                      FStar_TypeChecker_Env.use_bv_sorts =
                        (env.FStar_TypeChecker_Env.use_bv_sorts);
                      FStar_TypeChecker_Env.qtbl_name_and_index =
@@ -1847,6 +1858,8 @@ let (tc_decl' :
                                FStar_TypeChecker_Env.typeof_well_typed_tot_or_gtot_term
                                  =
                                  (env1.FStar_TypeChecker_Env.typeof_well_typed_tot_or_gtot_term);
+                               FStar_TypeChecker_Env.subtype_nosmt_force =
+                                 (env1.FStar_TypeChecker_Env.subtype_nosmt_force);
                                FStar_TypeChecker_Env.use_bv_sorts =
                                  (env1.FStar_TypeChecker_Env.use_bv_sorts);
                                FStar_TypeChecker_Env.qtbl_name_and_index =
@@ -2104,6 +2117,8 @@ let (tc_decl' :
                                   FStar_TypeChecker_Env.typeof_well_typed_tot_or_gtot_term
                                     =
                                     (env.FStar_TypeChecker_Env.typeof_well_typed_tot_or_gtot_term);
+                                  FStar_TypeChecker_Env.subtype_nosmt_force =
+                                    (env.FStar_TypeChecker_Env.subtype_nosmt_force);
                                   FStar_TypeChecker_Env.use_bv_sorts =
                                     (env.FStar_TypeChecker_Env.use_bv_sorts);
                                   FStar_TypeChecker_Env.qtbl_name_and_index =
@@ -2300,6 +2315,8 @@ let (tc_decl' :
                              FStar_TypeChecker_Env.typeof_well_typed_tot_or_gtot_term
                                =
                                (env.FStar_TypeChecker_Env.typeof_well_typed_tot_or_gtot_term);
+                             FStar_TypeChecker_Env.subtype_nosmt_force =
+                               (env.FStar_TypeChecker_Env.subtype_nosmt_force);
                              FStar_TypeChecker_Env.use_bv_sorts =
                                (env.FStar_TypeChecker_Env.use_bv_sorts);
                              FStar_TypeChecker_Env.qtbl_name_and_index =
@@ -2492,6 +2509,8 @@ let (tc_decl' :
                            FStar_TypeChecker_Env.typeof_well_typed_tot_or_gtot_term
                              =
                              (env1.FStar_TypeChecker_Env.typeof_well_typed_tot_or_gtot_term);
+                           FStar_TypeChecker_Env.subtype_nosmt_force =
+                             (env1.FStar_TypeChecker_Env.subtype_nosmt_force);
                            FStar_TypeChecker_Env.use_bv_sorts =
                              (env1.FStar_TypeChecker_Env.use_bv_sorts);
                            FStar_TypeChecker_Env.qtbl_name_and_index =
@@ -2644,6 +2663,8 @@ let (tc_decl' :
                            FStar_TypeChecker_Env.typeof_well_typed_tot_or_gtot_term
                              =
                              (env1.FStar_TypeChecker_Env.typeof_well_typed_tot_or_gtot_term);
+                           FStar_TypeChecker_Env.subtype_nosmt_force =
+                             (env1.FStar_TypeChecker_Env.subtype_nosmt_force);
                            FStar_TypeChecker_Env.use_bv_sorts =
                              (env1.FStar_TypeChecker_Env.use_bv_sorts);
                            FStar_TypeChecker_Env.qtbl_name_and_index =
@@ -2838,6 +2859,8 @@ let (tc_decl' :
                             FStar_TypeChecker_Env.typeof_well_typed_tot_or_gtot_term
                               =
                               (env.FStar_TypeChecker_Env.typeof_well_typed_tot_or_gtot_term);
+                            FStar_TypeChecker_Env.subtype_nosmt_force =
+                              (env.FStar_TypeChecker_Env.subtype_nosmt_force);
                             FStar_TypeChecker_Env.use_bv_sorts =
                               (env.FStar_TypeChecker_Env.use_bv_sorts);
                             FStar_TypeChecker_Env.qtbl_name_and_index =
@@ -2968,6 +2991,8 @@ let (tc_decl' :
                                FStar_TypeChecker_Env.typeof_well_typed_tot_or_gtot_term
                                  =
                                  (env.FStar_TypeChecker_Env.typeof_well_typed_tot_or_gtot_term);
+                               FStar_TypeChecker_Env.subtype_nosmt_force =
+                                 (env.FStar_TypeChecker_Env.subtype_nosmt_force);
                                FStar_TypeChecker_Env.use_bv_sorts =
                                  (env.FStar_TypeChecker_Env.use_bv_sorts);
                                FStar_TypeChecker_Env.qtbl_name_and_index =
@@ -3157,6 +3182,8 @@ let (tc_decl' :
                                FStar_TypeChecker_Env.typeof_well_typed_tot_or_gtot_term
                                  =
                                  (env.FStar_TypeChecker_Env.typeof_well_typed_tot_or_gtot_term);
+                               FStar_TypeChecker_Env.subtype_nosmt_force =
+                                 (env.FStar_TypeChecker_Env.subtype_nosmt_force);
                                FStar_TypeChecker_Env.use_bv_sorts =
                                  (env.FStar_TypeChecker_Env.use_bv_sorts);
                                FStar_TypeChecker_Env.qtbl_name_and_index =
@@ -3436,6 +3463,8 @@ let (add_sigelt_to_env :
                        FStar_TypeChecker_Env.typeof_well_typed_tot_or_gtot_term
                          =
                          (env1.FStar_TypeChecker_Env.typeof_well_typed_tot_or_gtot_term);
+                       FStar_TypeChecker_Env.subtype_nosmt_force =
+                         (env1.FStar_TypeChecker_Env.subtype_nosmt_force);
                        FStar_TypeChecker_Env.use_bv_sorts =
                          (env1.FStar_TypeChecker_Env.use_bv_sorts);
                        FStar_TypeChecker_Env.qtbl_name_and_index =
@@ -3540,6 +3569,8 @@ let (add_sigelt_to_env :
                        FStar_TypeChecker_Env.typeof_well_typed_tot_or_gtot_term
                          =
                          (env1.FStar_TypeChecker_Env.typeof_well_typed_tot_or_gtot_term);
+                       FStar_TypeChecker_Env.subtype_nosmt_force =
+                         (env1.FStar_TypeChecker_Env.subtype_nosmt_force);
                        FStar_TypeChecker_Env.use_bv_sorts =
                          (env1.FStar_TypeChecker_Env.use_bv_sorts);
                        FStar_TypeChecker_Env.qtbl_name_and_index =
@@ -3644,6 +3675,8 @@ let (add_sigelt_to_env :
                        FStar_TypeChecker_Env.typeof_well_typed_tot_or_gtot_term
                          =
                          (env1.FStar_TypeChecker_Env.typeof_well_typed_tot_or_gtot_term);
+                       FStar_TypeChecker_Env.subtype_nosmt_force =
+                         (env1.FStar_TypeChecker_Env.subtype_nosmt_force);
                        FStar_TypeChecker_Env.use_bv_sorts =
                          (env1.FStar_TypeChecker_Env.use_bv_sorts);
                        FStar_TypeChecker_Env.qtbl_name_and_index =
@@ -3748,6 +3781,8 @@ let (add_sigelt_to_env :
                        FStar_TypeChecker_Env.typeof_well_typed_tot_or_gtot_term
                          =
                          (env1.FStar_TypeChecker_Env.typeof_well_typed_tot_or_gtot_term);
+                       FStar_TypeChecker_Env.subtype_nosmt_force =
+                         (env1.FStar_TypeChecker_Env.subtype_nosmt_force);
                        FStar_TypeChecker_Env.use_bv_sorts =
                          (env1.FStar_TypeChecker_Env.use_bv_sorts);
                        FStar_TypeChecker_Env.qtbl_name_and_index =
@@ -4108,6 +4143,8 @@ let (tc_partial_modul :
              (env.FStar_TypeChecker_Env.universe_of);
            FStar_TypeChecker_Env.typeof_well_typed_tot_or_gtot_term =
              (env.FStar_TypeChecker_Env.typeof_well_typed_tot_or_gtot_term);
+           FStar_TypeChecker_Env.subtype_nosmt_force =
+             (env.FStar_TypeChecker_Env.subtype_nosmt_force);
            FStar_TypeChecker_Env.use_bv_sorts =
              (env.FStar_TypeChecker_Env.use_bv_sorts);
            FStar_TypeChecker_Env.qtbl_name_and_index =
@@ -4354,6 +4391,8 @@ let (check_module :
                (env.FStar_TypeChecker_Env.universe_of);
              FStar_TypeChecker_Env.typeof_well_typed_tot_or_gtot_term =
                (env.FStar_TypeChecker_Env.typeof_well_typed_tot_or_gtot_term);
+             FStar_TypeChecker_Env.subtype_nosmt_force =
+               (env.FStar_TypeChecker_Env.subtype_nosmt_force);
              FStar_TypeChecker_Env.use_bv_sorts =
                (env.FStar_TypeChecker_Env.use_bv_sorts);
              FStar_TypeChecker_Env.qtbl_name_and_index =
