src/fstar/FStar.Universal.fst
@@ -124,6 +124,7 @@ let init_env deps : TcEnv.env =
         TcTerm.typeof_tot_or_gtot_term
         TcTerm.typeof_tot_or_gtot_term_fastpath
         TcTerm.universe_of
+        Rel.subtype_nosmt_force
         solver
         Const.prims_lid
         (NBE.normalize
